Leansubst/Basic.lean
@@ -1,0 +1,262 @@
+import Std.Data.Nat.Lemmas
+import Leansubst.Defs
+
+/-!
+  This file contains equational lemmas related to `Expr`, `Subst`, `ES` and `SE`.
+-/
+
+namespace Leansubst.Subst'
+
+variable {σ : Type}
+variable (s t u : Subst σ)
+variable (i : Nat) (x : σ)
+variable (e : Expr σ) (es : List (Expr σ))
+
+local notation:arg "⟦" a "⟧" => Quotient.mk _ a
+
+def up : Nat → Subst' σ → Subst' σ
+  | 0,     s => s
+  | i + 1, s => cons (.var 0) (comp (up i s) (shift 1))
+
+theorem get_up_low (i j k : Nat) (h : k < j) : (up j (@shift σ i)).get k = .var k := by
+  induction j generalizing k with
+  | zero => intros; contradiction
+  | succ j ih =>
+    cases Nat.eq_or_lt_of_le (Nat.le_of_lt_succ h) with
+    | inl h' =>
+      subst h'; rw [up]
+      cases k with
+      | zero => rfl
+      | succ k => rw [get, comp_def, ih k (Nat.lt_succ_self _), apply]
+    | inr h' =>
+      rw [up]
+      cases k with
+      | zero => rfl
+      | succ k =>
+        specialize ih _ (Nat.le_of_lt_succ h)
+        rw [get, comp_def, ih, apply]
+
+theorem get_up_high (i j k : Nat) (h : j ≤ k) : (up j (@shift σ i)).get k = .var (k + i) := by
+  have ⟨d, hd⟩ := Nat.le.dest h; clear h
+  induction j generalizing k d with
+  | zero => rfl
+  | succ j ih =>
+    rw [up]
+    cases k with
+    | zero => cases d <;> contradiction
+    | succ k =>
+      rw [get, comp_def]
+      rw [Nat.succ_add] at hd; injection hd with hd
+      rw [ih _ _ hd, apply, Nat.succ_add]
+
+theorem comp_eqv_comps (i j : Nat) : comp (up j (shift i)) (shift 1) ≈ (comps (up j (shift i)) 1 : Subst' σ) := by
+  intros k
+  rw [comp_def, comps_def]
+  cases Nat.lt_sum_ge k j with
+  | inl h =>
+    rw [get_up_low _ _ _ h, apply, applys]
+    split
+    case inl _ => rfl
+    case inr h => exact (h (Nat.zero_le _)).elim
+  | inr h =>
+    rw [get_up_high _ _ _ h, apply, applys]
+    split
+    case inl _ => rfl
+    case inr h => exact (h (Nat.zero_le _)).elim
+
+/-- We have to show that `applys` actually agrees with `apply shift`. -/
+theorem applys_def (i j : Nat) : applys j i e = apply (up j (shift i)) e := by
+  revert j
+  -- Induction on `e`.
+  apply @Expr.recOn _
+    (fun e => ∀ j, applys j i e = apply (up j (shift i)) e)
+    (List.foldr (fun e etc => (∀ j, applys j i e = apply (up j (shift i)) e) ∧ etc) True)
+    <;> intros <;> try trivial
+  case var k j =>
+    induction j generalizing k with
+    | zero =>
+      rw [up, applys]
+      split
+      case inl _ => rw [apply]
+      case inr h => exact (h (Nat.zero_le _)).elim
+    | succ j ih =>
+      simp only [up, applys, apply_var] at *
+      cases k with
+      | zero => (split <;> try contradiction); rfl
+      | succ k =>
+        simp only [get, comp_def, ← ih]
+        split <;> rename_i h
+        rotate_right; have h : ¬j ≤ k := fun h' => (h (Nat.succ_le_succ h')).elim
+        rotate_right; have h := Nat.le_of_succ_le_succ h
+        all_goals (split <;> try contradiction)
+        case inl => rw [apply, Nat.succ_add]
+        case inr => rw [apply]
+  case binder e ih j =>
+    rw [applys, apply, ih, up]
+    congr 1
+    have h := comp_eqv_comps i j (σ := σ)
+    have h' : (.cons (.var 0) ⟦comp (up j (shift i)) (shift 1)⟧ : Subst σ) e =
+              (.cons (.var 0) ⟦comps (up j (shift i)) 1⟧ : Subst σ) e := by rw [Quotient.sound h]
+    exact h'
+  case node x es ih j =>
+    induction es with
+    | nil => rw [applys, apply, apply.nested]; rfl
+    | cons h' t' ih' =>
+      rw [List.foldr] at ih
+      rw [applys, applys.nested, apply, apply.nested]
+      congr
+      . exact ih.left _
+      . specialize ih' ih.right
+        rw [applys, apply] at ih'
+        injection ih'
+
+end Subst'
+
+namespace Subst
+
+@[simp] theorem shift_wrap (n : Nat) : ⟦Subst'.shift n⟧ = Subst.shift σ n := rfl
+@[simp] theorem cons_wrap (e : Expr σ) (s : Subst' σ) : ⟦Subst'.cons e s⟧ = Subst.cons e ⟦s⟧ := rfl
+@[simp] theorem id_wrap : ⟦Subst'.id σ⟧ = Subst.id σ := rfl
+
+@[simp] theorem get_wrap (s : Subst' σ) (i : Nat) : Subst'.get s i = Subst.get ⟦s⟧ i := rfl
+@[simp] theorem apply_wrap (s : Subst' σ) : Subst'.apply s = Subst.apply ⟦s⟧ := rfl
+@[simp] theorem comps_wrap (s : Subst' σ) (n : Nat) : ⟦Subst'.comps s n⟧ = Subst.comps ⟦s⟧ n := rfl
+@[simp] theorem comp_wrap (s t : Subst' σ) : ⟦Subst'.comp s t⟧ = Subst.comp ⟦s⟧ ⟦t⟧ := rfl
+
+variable {σ : Type}
+variable (s t u : Subst σ)
+variable (i : Nat) (x : σ)
+variable (e : Expr σ) (es : List (Expr σ))
+
+@[simp]
+theorem get_zero : (cons e s).get 0 = e := by
+  induction s using Quotient.inductionOn
+  rw [← cons_wrap, ← get_wrap]
+  rfl
+
+@[simp]
+theorem get_succ : (cons e s).get (i + 1) = s.get i := by
+  induction s using Quotient.inductionOn
+  rw [← cons_wrap, ← get_wrap]
+  rfl
+
+@[simp]
+theorem shift_expand : shift σ (i + 1 + 1) = comp (shift σ (i + 1)) (shift σ 1) := by
+  simp only [← shift_wrap, ← comp_wrap]
+  apply Quotient.sound
+  intros j
+  rfl
+
+@[simp]
+theorem comps_expand : comps s i = comp s (shift σ i) := by
+  induction s using Quotient.inductionOn
+  rw [← comps_wrap, ← shift_wrap, ← comp_wrap]
+  apply Quotient.sound
+  intros j
+  rw [Subst'.comps_def, Subst'.comp_def, Subst'.applys_def]
+  rfl
+
+@[simp]
+theorem apply_var : s (.var i) = s.get i := by
+  induction s using Quotient.inductionOn
+  rw [← apply_wrap, ← get_wrap, Subst'.apply_var]
+
+@[simp]
+theorem apply_binder : s (.binder e) = .binder ((cons (.var 0) (comp s (shift σ 1))) e) := by
+  induction s using Quotient.inductionOn
+  rw [← apply_wrap, Subst'.apply]
+  simp
+
+@[simp]
+theorem apply_node : s (.node x es) = .node x (es.map s) := by
+  induction s using Quotient.inductionOn
+  induction es with
+  | nil => rw [List.map, ← apply_wrap, Subst'.apply, Subst'.apply.nested]
+  | cons h t ih =>
+    rw [List.map, ← apply_wrap, Subst'.apply, Subst'.apply.nested]
+    rw [← apply_wrap, Subst'.apply] at ih
+    congr; injection ih
+
+@[simp]
+theorem apply_apply : t (s e) = (comp s t) e := by
+  induction s using Quotient.inductionOn; rename_i s
+  induction t using Quotient.inductionOn; rename_i t
+  simp only [← comp_wrap, ← apply_wrap]
+  sorry
+
+@[simp]
+theorem id_apply : (id σ) e = e := by
+  rw [← id_wrap, ← apply_wrap]
+  rw [Subst'.id]
+  sorry
+
+@[simp]
+theorem id_comp : comp (id σ) s = s := by
+  induction s using Quotient.inductionOn
+  rw [← id_wrap, ← comp_wrap]
+  apply Quotient.sound
+  intros j
+  rw [Subst'.id, Subst'.comp_def, Subst'.get, Subst'.apply_var]
+  rfl
+
+@[simp]
+theorem comp_id : comp s (id σ) = s := by
+  induction s using Quotient.inductionOn
+  rw [← id_wrap, ← comp_wrap]
+  apply Quotient.sound
+  intros j
+  rw [Subst'.comp_def]
+  sorry
+
+@[simp]
+theorem shift_comp_cons : comp (shift σ 1) (cons e s) = s := by
+  induction s using Quotient.inductionOn
+  rw [← cons_wrap, ← shift_wrap, ← comp_wrap]
+  apply Quotient.sound
+  intros j
+  rw [Subst'.comp_def, Subst'.get, Subst'.apply, Subst'.apply_var]
+
+@[simp]
+theorem cons_comp : comp (cons e s) t = cons (s e) (comp s t) := by
+  induction s using Quotient.inductionOn
+  induction t using Quotient.inductionOn
+  simp only [← apply_wrap, ← cons_wrap, ← comp_wrap]
+  apply Quotient.sound
+  intros j
+  sorry
+
+@[simp]
+theorem comp_assoc : comp (comp s t) u = comp s (comp t u) := by
+  induction s using Quotient.inductionOn
+  induction t using Quotient.inductionOn
+  induction u using Quotient.inductionOn
+  simp only [← comp_wrap]
+  apply Quotient.sound
+  intros j
+  simp only [Subst'.comp_def, Subst'.apply]
+  sorry
+
+@[simp]
+theorem apply_zero_cons_shift_comp : cons (s (.var 0)) (comp (shift σ 1) s) = s := by
+  induction s using Quotient.inductionOn
+  rw [← shift_wrap, ← apply_wrap, ← comp_wrap, ← cons_wrap]
+  apply Quotient.sound
+  intros j
+  rw [Subst'.apply_var]
+  sorry
+
+@[simp]
+theorem zero_cons_shift : cons (.var 0) (shift σ 1) = id σ := by
+  rw [← shift_wrap, ← id_wrap, ← cons_wrap]
+  apply Quotient.sound
+  intros j
+  cases j with
+  | zero => rfl
+  | succ => rfl
+
+/-
+example : comp (shift σ 1) (id σ) = shift σ 1 := by
+  simp
+-/
+
+end Leansubst.Subst
